crates/move-prover-boogie-backend/src/boogie_backend/prelude/native.bpl
@@ -932,15 +932,18 @@ procedure {:inline 2} {{impl.fun_remove}}{{DF_S}}(m: $Mutation ({{Type}}), k: {{
 procedure {:inline 2} {{impl.fun_remove_if_exists}}{{DF_S}}(m: $Mutation ({{Type}}), k: {{K}}) returns (v: $1_option_Option'{{instance.1.suffix}}', m': $Mutation({{Type}})) {
     var enc_k: int;
     var t: {{Type}};
+    var val: {{V}};
     enc_k := {{ENC}}(k);
     t := $Dereference(m);
     if (ContainsTable(t->$dynamic_fields{{S}}, enc_k)) {
+        val := GetTable(t->$dynamic_fields{{S}}, enc_k);
+        assume $IsValid{{SV}}(val);
         m' := $UpdateMutation(m, $Update'{{Type}}'_dynamic_fields{{S}}(t, RemoveTable(t->$dynamic_fields{{S}}, enc_k)));
+        v := $1_option_Option{{SV}}(MakeVec1(val));
     } else {
         m' := m;
+        v := $1_option_Option{{SV}}(EmptyVec());
     }
-    // v is havoc'd - the important effect is the removal from dynamic_fields
-    havoc v;
 }
 {%- endif %}
 
